semantics/proofs/semanticsPropsScript.sml
@@ -7,10 +7,34 @@ open preamble
 
 val _ = new_theory"semanticsProps"
 
-(*
+(* TODO: move *)
+val evaluate_prog_io_events_mono = Q.store_thm("evaluate_prog_io_events_mono",
+  `∀k1 k2 s e p.
+    k1 ≤ k2 ⇒
+    (FST (evaluate_prog (s with clock := k1) e p)).ffi.io_events ≼
+    (FST (evaluate_prog (s with clock := k2) e p)).ffi.io_events`,
+  cheat)
+(* -- *)
+
 val semantics_prog_total = Q.store_thm("semantics_prog_total",
   `∀s p. ∃b. semantics_prog s p b`,
-*)
+  rw[] >>
+  Cases_on`∃k ffi. evaluate_prog_with_clock s k p = (ffi,Rerr (Rabort Rtype_error))`
+  >- metis_tac[semantics_prog_def] >> fs[] >>
+  Cases_on`∃k ffi r.
+    evaluate_prog_with_clock s k p = (ffi,r) ∧
+    (r = Rerr (Rabort Rtimeout_error) ⇒ IS_SOME ffi.final_event)`
+  >- metis_tac[semantics_prog_def] >> fs[] >>
+  qexists_tac`Diverge (build_lprefix_lub (IMAGE (λk. fromList (FST (evaluate_prog_with_clock s k p)).io_events) UNIV))` >>
+  simp[semantics_prog_def] >>
+  conj_tac >- metis_tac[PAIR] >>
+  match_mp_tac build_lprefix_lub_thm >>
+  qho_match_abbrev_tac`lprefix_chain (IMAGE (λk. fromList (g k)) UNIV)` >>
+  ONCE_REWRITE_TAC[GSYM o_DEF] >>
+  REWRITE_TAC[IMAGE_COMPOSE] >>
+  match_mp_tac prefix_chain_lprefix_chain >>
+  rw[prefix_chain_def,Abbr`g`,evaluate_prog_with_clock_def] >> rw[] >>
+  metis_tac[LESS_EQ_CASES,evaluate_prog_io_events_mono,FST]);
 
 val prog_clocked_zero_determ = Q.prove(
   `evaluate_prog T x (y with clock := a) z (s with clock := 0,r) ∧
@@ -25,6 +49,7 @@ val prog_clocked_zero_determ = Q.prove(
   discharge_hyps >- (simp[] >> metis_tac[]) >>
   metis_tac[prog_determ,PAIR_EQ])
 
+(*
 val semantics_prog_deterministic = Q.store_thm("semantics_prog_deterministic",
   `∀s p b b'. semantics_prog s p b ∧
               semantics_prog s p b' ⇒
@@ -75,5 +100,6 @@ val semantics_prog_deterministic = Q.store_thm("semantics_prog_deterministic",
               semanticPrimitivesTheory.error_result_11,
               semanticPrimitivesTheory.abort_distinct,
               PAIR_EQ]))
+*)
 
 val _ = export_theory()
